src/syntax/FStar.Syntax.Util.fst
@@ -1287,11 +1287,11 @@ let exp_int s : term = mk (Tm_constant (Const_int (s,None))) dummyRange
 let exp_char c : term = mk (Tm_constant (Const_char c)) dummyRange
 let exp_string s : term = mk (Tm_constant (Const_string (s, dummyRange))) dummyRange
 
-let fvar_const l = fvar l delta_constant None
+let fvar_const l = fvar_with_dd l delta_constant None
 let tand    = fvar_const PC.and_lid
 let tor     = fvar_const PC.or_lid
-let timp    = fvar PC.imp_lid (Delta_constant_at_level 1) None //NS delta: wrong? level 2
-let tiff    = fvar PC.iff_lid (Delta_constant_at_level 2) None //NS delta: wrong? level 3
+let timp    = fvar_with_dd PC.imp_lid (Delta_constant_at_level 1) None //NS delta: wrong? level 2
+let tiff    = fvar_with_dd PC.iff_lid (Delta_constant_at_level 2) None //NS delta: wrong? level 3
 let t_bool  = fvar_const PC.bool_lid
 let b2t_v   = fvar_const PC.b2t_lid
 let t_not   = fvar_const PC.not_lid
@@ -1307,7 +1307,7 @@ let rename_let_attr = fvar_const PC.rename_let_attr
 let t_ctx_uvar_and_sust = fvar_const PC.ctx_uvar_and_subst_lid
 let t_universe_uvar     = fvar_const PC.universe_uvar_lid
 
-let t_dsl_tac_typ = fvar PC.dsl_tac_typ_lid (Delta_constant_at_level 1) None
+let t_dsl_tac_typ = fvar PC.dsl_tac_typ_lid None
 
 
 let mk_conj_opt phi1 phi2 = match phi1 with
@@ -1317,7 +1317,7 @@ let mk_binop op_t phi1 phi2 = mk (Tm_app {hd=op_t; args=[as_arg phi1; as_arg phi
 let mk_neg phi = mk (Tm_app {hd=t_not; args=[as_arg phi]}) phi.pos
 let mk_conj phi1 phi2 = mk_binop tand phi1 phi2
 let mk_conj_l phi = match phi with
-    | [] -> fvar PC.true_lid delta_constant None //NS delta: wrong, see a t_true
+    | [] -> fvar_with_dd PC.true_lid delta_constant None //NS delta: wrong, see a t_true
     | hd::tl -> List.fold_right mk_conj tl hd
 let mk_disj phi1 phi2 = mk_binop tor phi1 phi2
 let mk_disj_l phi = match phi with
@@ -1362,9 +1362,9 @@ let mk_has_type t x t' =
     let t_has_type = mk (Tm_uinst(t_has_type, [U_zero; U_zero])) dummyRange in
     mk (Tm_app {hd=t_has_type; args=[iarg t; as_arg x; as_arg t']}) dummyRange
 
-let tforall  = fvar PC.forall_lid (Delta_constant_at_level 1) None //NS delta: wrong level 2
-let texists  = fvar PC.exists_lid (Delta_constant_at_level 1) None //NS delta: wrong level 2
-let t_haseq   = fvar PC.haseq_lid delta_constant None //NS delta: wrong Delta_abstract (Delta_constant_at_level 0)?
+let tforall  = fvar_with_dd PC.forall_lid (Delta_constant_at_level 1) None //NS delta: wrong level 2
+let texists  = fvar_with_dd PC.exists_lid (Delta_constant_at_level 1) None //NS delta: wrong level 2
+let t_haseq   = fvar_with_dd PC.haseq_lid delta_constant None //NS delta: wrong Delta_abstract (Delta_constant_at_level 0)?
 
 let decidable_eq = fvar_const PC.op_Eq
 let mk_decidable_eq t e1 e2 =
@@ -1438,11 +1438,11 @@ let if_then_else b t1 t2 =
 // Operations on squashed and other irrelevant/sub-singleton types
 //////////////////////////////////////////////////////////////////////////////////////
 let mk_squash u p =
-    let sq = fvar PC.squash_lid (Delta_constant_at_level 1) None in //NS delta: ok
+    let sq = fvar_with_dd PC.squash_lid (Delta_constant_at_level 1) None in //NS delta: ok
     mk_app (mk_Tm_uinst sq [u]) [as_arg p]
 
 let mk_auto_squash u p =
-    let sq = fvar PC.auto_squash_lid (Delta_constant_at_level 2) None in //NS delta: ok
+    let sq = fvar_with_dd PC.auto_squash_lid (Delta_constant_at_level 2) None in //NS delta: ok
     mk_app (mk_Tm_uinst sq [u]) [as_arg p]
 
 let un_squash t =
@@ -2453,9 +2453,7 @@ let is_erased_head (t:term) : option (universe & term) =
     None
 
 let apply_reveal (u:universe) (ty:term) (v:term) =
-  let head = fvar (Ident.set_lid_range PC.reveal v.pos)
-                  (Delta_constant_at_level 1)
-                   None in
+  let head = fvar (Ident.set_lid_range PC.reveal v.pos) None in
   mk_Tm_app (mk_Tm_uinst head [u])
             [iarg ty; as_arg v]
             v.pos
